---
usemathjax: true
---

[[Contrapositive]] of [[Conditional Statement]] $p \to q$ will be [[Equivalent]] to original statement. So proving the contrapositive ($\neg q \to \neg p$) will also prove original conditional statement.

* We assume the original statement is false, this is our new statement.
* Then we reach [[Negation]] of [[Conclusion]] (in new statement).
* This proves that [[Hypothesis]] was also false (in new statement.
* Thus, original statement was true.

### Subtopics
- [[Vacuous Proofs]]
- [[Trivial Proofs]]